examples/opaque/server_proofs.v
@@ -11,26 +11,60 @@ From cryptis.examples.opaque Require Import impl shared.
 
 From iris.base_logic.lib Require Import invariants.
 
+From cryptis.lib Require Import term_set.
+
 Set Implicit Arguments.
 Unset Strict Implicit.
 Unset Printing Implicit Defensive.
 
 Section Opaque.
 
-(* Context `{!cryptisGS Σ, !heapGS Σ, !spawnG Σ}. *)
-Context `{!cryptisGS Σ, !heapGS Σ, !iso_dhGS Σ, !storeGS Σ, !tlockG Σ}.
+Context `{!cryptisGS Σ, !heapGS Σ, !spawnG Σ}.
 
 Notation iProp := (iProp Σ).
 
+Definition opaque_file (file : term) : iProp :=
+  ∃ k_s p_s P_s P_u envelope,
+    ⌜file = Spec.of_list [k_s; p_s; P_s; P_u; envelope]⌝
+    ∗ minted k_s ∗ minted p_s ∗ public P_s ∗ public P_u ∗ public envelope.
+
 Definition opaque_db (db : gmap term term) : iProp :=
 [∗ map] (k : term) ↦ (file : term) ∈ db,
-    public k ∗ (∃ k_s p_s P_s P_u envelope,
-                   ⌜file = Spec.of_list [k_s; p_s; P_s; P_u; envelope]⌝
-                  ∗ minted k_s ∗ minted p_s ∗ public P_s ∗ public P_u ∗ public envelope).
+public k ∗ opaque_file file.
 
-Lemma list_inv 
+Lemma wp_make_file (pw : term) :
+{{{ cryptis_ctx ∗ minted pw }}}
+Server.make_file pw
+{{{ file , RET file ; True }}}.
+Proof.
+  iIntros "%ϕ [#cryptis Hmintedpw] post".
+  wp_lam.
+  wp_apply (wp_mk_nonce (fun _ => False)%I (fun _ => False)%I) => //.
+  iIntros "%k_s %Hnoncek_s Hmintedk_s Hprivatek_s H!eqk_s Htokenk_s".
+  wp_pures.
+  wp_lam.
+  wp_pures.
+  wp_apply wp_H' => //.
+  unfold hash_result.
+  iIntros "_".
+  wp_pures.
+  wp_apply wp_texp.
+  wp_list.
+  wp_apply wp_H => //.
+  iIntros "_".
+  wp_apply wp_derive_senc_key.
+  wp_pures.
+  wp_apply (wp_mk_nonce (fun _ => False)%I (fun _ => False)%I) => //.
+  iIntros "%p_s %Hnoncep_s Hmintedp_s Hprivatep_s H!eqp_s Htokenp_s".
+  wp_pures.
+  wp_apply (wp_mk_nonce (fun _ => False)%I (fun _ => False)%I) => //.
+  iIntros "%p_u %Hnoncep_u Hmintedp_u Hprivatep_u H!eqp_u Htokenp_u".
+  wp_pures.
+  wp_apply wp_texp. wp_pures.
+  wp_apply wp_texp. wp_pures.
+Admitted.
 
-Lemma wp_server_session (db c : term) (alist : gmap term term): 
+Lemma wp_server_session (db c : term) (alist : gmap term term) : 
 cryptis_ctx -∗
 channel c -∗
 AList.is_alist db (repr <$> alist) -∗
@@ -54,28 +88,17 @@ Proof.
   iIntros "!> Hdb". rewrite lookup_fmap.
   case db_uid: (alist !! uid) => [file|]; wp_pures.
   2: by iModIntro.
-  
   iDestruct ("Hmapcontents" $! uid file with "[//]") as
-    "[_ (%k_s' & %p_s' & %P_s' & %P_u' & %envelope' &
-        %e' & Hmk_s & Hmp_s & HpP_s & HpP_u & Hpenvelope)]".
-
+    "[_ (%k_s & %p_s & %P_s & %P_u & %envelope &
+        %e & Hmk_s & Hmp_s & HpP_s & HpP_u & Hpenvelope)]".
   repeat rewrite subst_list_match /=.
-
-  
-wp_apply wp_list_of_term.
-rewrite e'.
-rewrite Spec.
-
-  
-2: wp_pures.
-  2: by iModIntro.  
+  wp_apply wp_list_of_term.
+  rewrite e.
+  rewrite Spec.of_listK.
   wp_pures.
-
-  unfold repr_list.
-
-  repeat rewrite subst_list_match /=.
-  
-wp_list_match => [k_s p_s P_s P_u envelope _ | ].
+  rewrite subst_list_match /=.
+  wp_list_match => [k_s' p_s' P_s' P_u' envelope' e' | ].
+  inversion e'. subst. clear e'.
   2: intro H; wp_pures; by iModIntro.
   wp_apply (wp_mk_nonce (fun _ => False)%I (fun _ => False)%I).
   1: iAssumption.
@@ -106,7 +129,6 @@ wp_list_match => [k_s p_s P_s P_u envelope _ | ].
   wp_list.
   wp_term_of_list.
   wp_pures.
-  rewrite Hm1eq.
   rewrite public_of_list.
   simpl.
   iDestruct "Hpubm1" as "[Hpubuid [Hpubα [HpubX_u _]]]".
@@ -124,20 +146,6 @@ wp_list_match => [k_s p_s P_s P_u envelope _ | ].
   by iApply minted_TInt.
   iApply "H!eqx_s". iNext. iModIntro. admit.
   admit.
-  iApply public_THash.
-  iRight. iSplit.
-  iApply minted_tag. iApply minted_of_list. do !iSplit => //.
-  iApply minted_THash. iApply minted_tag. iApply minted_of_list. do !iSplit => //.
-  iApply minted_TExp.
-  admit.
-  admit.
-  iApply minted_TExp.
-  admit.
-  admit.
-  iApply minted_THash. iApply minted_tag. iApply minted_of_list. do !iSplit => //.
-  admit.
-  admit.
-  admit.
   wp_pures.
   wp_apply (wp_recv with "Hc").
   iIntros "%m3 #Hm3pub".
@@ -150,7 +158,6 @@ wp_list_match => [k_s p_s P_s P_u envelope _ | ].
   wp_list.
   wp_pures.
   by iModIntro.
-Admitted.
-  
+Admitted.  
 
 End Opaque.
